Correctness of the original semantics with regard to the resourced semantics

Launchbury/HSemUpd.thy
@@ -1,5 +1,5 @@
 theory HSemUpd
-  imports "HeapToEnv" "DistinctVars-Nominal"  "HOLCF-Fix-Join-Nominal" "FMap-Utils"
+  imports "HeapToEnv" "DistinctVars-Nominal"  "HOLCF-Fix-Join-Nominal" "FMap-Utils" "HasESem"
 begin
 
 subsubsection {* A locale for heap semantics, abstract in the expression semantics *}
@@ -9,23 +9,22 @@ This theory follows closely the theory @{text HSem}, but uses right-sided update
 instead of least upper bounds. 
 *}
 
-locale has_ESem =
-  fixes ESem :: "'exp::pt \<Rightarrow> 'var::{cont_pt,at_base} f\<rightharpoonup> 'value \<Rightarrow> 'value::{pure_cpo,Nonempty_Meet_cpo,pcpo}" ("\<lbrakk> _ \<rbrakk>\<^bsub>_\<^esub>"  [60,60] 60)
+context has_ESem
 begin
 
-definition HSem :: "('var \<times> 'exp) list \<Rightarrow> 'var f\<rightharpoonup> 'value \<Rightarrow> 'var f\<rightharpoonup> 'value" ("\<lbrace>_\<rbrace>_"  [60,60] 60)
+definition UHSem :: "('var \<times> 'exp) list \<Rightarrow> 'var f\<rightharpoonup> 'value \<Rightarrow> 'var f\<rightharpoonup> 'value" ("\<lbrace>_\<rbrace>_"  [60,60] 60)
   where
   "\<lbrace>h\<rbrace>\<rho> = 
     (if (\<forall> e \<in> snd `set h. cont (ESem e))
      then  fix_on' (f\<emptyset>\<^bsub>[fdom \<rho> \<union> heapVars h]\<^esub>) (\<lambda> \<rho>'. \<rho> f++ heapToEnv h (\<lambda> e. \<lbrakk>e\<rbrakk>\<^bsub>\<rho>'\<^esub>))
      else (f\<emptyset>\<^bsub>[fdom \<rho> \<union> heapVars h]\<^esub>))"
 
-lemma HSem_def'':
+lemma UHSem_def'':
   assumes "\<And> e. e \<in> snd ` set h \<Longrightarrow> cont (ESem e)"
   shows "\<lbrace>h\<rbrace>\<rho> = fix_on' (f\<emptyset>\<^bsub>[fdom \<rho> \<union> heapVars h]\<^esub>) (\<lambda> \<rho>'. \<rho> f++ heapToEnv h (\<lambda> e. \<lbrakk>e\<rbrakk>\<^bsub>\<rho>'\<^esub>))"
-  unfolding HSem_def using assms by metis
+  unfolding UHSem_def using assms by metis
 
-lemma fix_on_cond_HSem':
+lemma fix_on_cond_UHSem':
   assumes cont: "\<And> e. e \<in> snd ` set h \<Longrightarrow> cont (ESem e)"
   shows "fix_on_cond {x. f\<emptyset>\<^bsub>[fdom \<rho> \<union> heapVars h]\<^esub> \<sqsubseteq> x}
           (f\<emptyset>\<^bsub>[fdom \<rho> \<union> heapVars h]\<^esub>) (\<lambda>\<rho>'. \<rho> f++ heapToEnv h (\<lambda>e. \<lbrakk>e\<rbrakk>\<^bsub>\<rho>'\<^esub>))"
@@ -40,33 +39,33 @@ lemma fix_on_cond_HSem':
 
 subsubsection {* Continuity *}
 
-lemma HSem_monofun'':
+lemma UHSem_monofun'':
   assumes cont: "\<And> e. e \<in> snd ` set h \<Longrightarrow> cont (ESem e)"
   assumes "\<rho> \<sqsubseteq> \<rho>'"
   shows "\<lbrace>h\<rbrace>\<rho> \<sqsubseteq> \<lbrace>h\<rbrace>\<rho>'"
-  apply (subst (1 2) HSem_def'')
+  apply (subst (1 2) UHSem_def'')
   apply (erule cont)
-  apply (rule fix_on_mono2[OF fix_on_cond_HSem'[OF cont] fix_on_cond_HSem'[OF cont]])
+  apply (rule fix_on_mono2[OF fix_on_cond_UHSem'[OF cont] fix_on_cond_UHSem'[OF cont]])
     apply assumption+
   apply (metis assms(2) below.r_refl fmap_below_dom)
   apply (rule fmap_add_mono[OF `\<rho> \<sqsubseteq> \<rho>'`])
   by (rule cont2monofunE[OF cont2cont_heapToEnv[OF cont]])
 
-lemma HSem_cont'':
+lemma UHSem_cont'':
   assumes cont: "\<And> e. e \<in> snd ` set h \<Longrightarrow> cont (ESem e)"
   assumes "chain Y"
   shows "\<lbrace>h\<rbrace>(\<Squnion> i. Y  i) = (\<Squnion> i. \<lbrace>h\<rbrace>(Y i))"
 proof-
   have fdoms:"\<And> i. fdom (Y i) = fdom (\<Squnion> i. Y i)" (is "\<And> _ .(_ = ?d)") by (metis chain_fdom `chain Y`) 
   show ?thesis
-    apply (subst (1 2) HSem_def'')
+    apply (subst (1 2) UHSem_def'')
     apply (erule cont)+
     unfolding fdoms
     proof (rule fix_on_cont[OF `chain Y`, where S = "{x . f\<emptyset>\<^bsub>[fdom (\<Squnion> i. Y i) \<union> heapVars h]\<^esub> \<sqsubseteq> x}"])
       show "cont (\<lambda>a b. a f++ heapToEnv h (\<lambda>e. \<lbrakk>e\<rbrakk>\<^bsub>b\<^esub>))"
         by (rule cont2cont_lambda[OF fmap_add_cont1])
       fix i
-        from fix_on_cond_HSem'[OF cont, where \<rho> = "Y i", unfolded fdoms]
+        from fix_on_cond_UHSem'[OF cont, where \<rho> = "Y i", unfolded fdoms]
         show "fix_on_cond {x. f\<emptyset>\<^bsub>[fdom (\<Squnion> i. Y i) \<union> heapVars h]\<^esub> \<sqsubseteq> x}
                (f\<emptyset>\<^bsub>[fdom (Lub Y) \<union> heapVars h]\<^esub>) (\<lambda>a. Y i f++ heapToEnv h (\<lambda>e. \<lbrakk>e\<rbrakk>\<^bsub>a\<^esub>))"
            by metis
@@ -74,30 +73,29 @@ proof-
 qed
 end
 
-locale has_cont_ESem = has_ESem +
-  assumes ESem_cont: "\<And> e. cont (ESem e)"
+context has_cont_ESem
 begin
 
-  lemma HSem_def':
+  lemma UHSem_def':
     shows "\<lbrace>h\<rbrace>\<rho> = fix_on' (f\<emptyset>\<^bsub>[fdom \<rho> \<union> heapVars h]\<^esub>) (\<lambda> \<rho>'. \<rho> f++ heapToEnv h (\<lambda> e. \<lbrakk>e\<rbrakk>\<^bsub>\<rho>'\<^esub>))"
-    unfolding HSem_def using ESem_cont by metis
+    unfolding UHSem_def using ESem_cont by metis
 
-  lemma fix_on_cond_HSem:
+  lemma fix_on_cond_UHSem:
     shows "fix_on_cond {x. f\<emptyset>\<^bsub>[fdom \<rho> \<union> heapVars h]\<^esub> \<sqsubseteq> x}
             (f\<emptyset>\<^bsub>[fdom \<rho> \<union> heapVars h]\<^esub>) (\<lambda>\<rho>'. \<rho> f++ heapToEnv h (\<lambda>e. \<lbrakk>e\<rbrakk>\<^bsub>\<rho>'\<^esub>))"
-    apply (rule fix_on_cond_HSem') using ESem_cont by metis
+    apply (rule fix_on_cond_UHSem') using ESem_cont by metis
 
 
 subsubsection {* Induction and other lemmas about @{term HSem} *}
 
-  lemma HSem_ind:
+  lemma UHSem_ind:
     assumes "adm P"
     assumes "P (f\<emptyset>\<^bsub>[fdom \<rho> \<union> heapVars h]\<^esub>)"
     assumes step: "\<And> y. fdom y = fdom \<rho> \<union> heapVars h \<Longrightarrow>
           P y \<Longrightarrow>  P (\<rho> f++ (heapToEnv h (\<lambda>e. \<lbrakk>e\<rbrakk>\<^bsub>y\<^esub>)))"
     shows "P (\<lbrace>h\<rbrace>\<rho>)"
-    unfolding HSem_def'
-    apply (rule fix_on_ind[OF fix_on_cond_HSem])
+    unfolding UHSem_def'
+    apply (rule fix_on_ind[OF fix_on_cond_UHSem])
     apply (rule adm_is_adm_on[OF `adm P`])
     apply fact
     apply (rule step)
@@ -105,12 +103,12 @@ subsubsection {* Induction and other lemmas about @{term HSem} *}
     apply assumption
     done
 
-  lemma HSem_below:
+  lemma UHSem_below:
     assumes [simp]:"fdom r = fdom \<rho> \<union> heapVars h" 
     assumes rho: "\<And>x. x \<in> fdom \<rho> \<Longrightarrow> x \<notin> heapVars h \<Longrightarrow> \<rho> f! x \<sqsubseteq> r f! x"
     assumes h: "\<And>x. x \<in> heapVars h \<Longrightarrow> \<lbrakk>the (map_of h x)\<rbrakk>\<^bsub>r\<^esub> \<sqsubseteq> r f! x"
-    shows "HSem h \<rho> \<sqsubseteq> r"
-  proof (rule HSem_ind)
+    shows "UHSem h \<rho> \<sqsubseteq> r"
+  proof (rule UHSem_ind)
     case goal1 show ?case by (auto intro: adm_is_adm_on)
     case goal2 show ?case by (simp add: to_bot_fmap_def)
     case (goal3 \<rho>')
@@ -123,7 +121,7 @@ subsubsection {* Induction and other lemmas about @{term HSem} *}
       done
   qed  
   
-  lemma parallel_HSem_ind:
+  lemma parallel_UHSem_ind:
     assumes "adm (\<lambda>\<rho>'. P (fst \<rho>') (snd \<rho>'))"
     assumes "P (f\<emptyset>\<^bsub>[fdom \<rho> \<union> heapVars h]\<^esub>) (f\<emptyset>\<^bsub>[fdom \<rho>2 \<union> heapVars h2]\<^esub>)"
     assumes step: "\<And>y z. fdom y = fdom \<rho> \<union> heapVars h \<Longrightarrow>
@@ -131,40 +129,40 @@ subsubsection {* Induction and other lemmas about @{term HSem} *}
             P y z \<Longrightarrow>
             P (\<rho> f++ (heapToEnv h (\<lambda>e. \<lbrakk>e\<rbrakk>\<^bsub>y\<^esub>))) (\<rho>2 f++ (heapToEnv h2 (\<lambda>e. \<lbrakk>e\<rbrakk>\<^bsub>z\<^esub>)))"
     shows "P (\<lbrace>h\<rbrace>\<rho>) (\<lbrace>h2\<rbrace>\<rho>2)"
-    unfolding HSem_def'
-    apply (rule parallel_fix_on_ind[OF fix_on_cond_HSem fix_on_cond_HSem])
+    unfolding UHSem_def'
+    apply (rule parallel_fix_on_ind[OF fix_on_cond_UHSem fix_on_cond_UHSem])
     apply (rule adm_is_adm_on[OF `adm _`])
     apply fact
     apply (rule step)
     apply simp+
     done
   
-  lemma HSem_eq:
+  lemma UHSem_eq:
     shows "\<lbrace>h\<rbrace>\<rho> = \<rho> f++ (heapToEnv h (\<lambda>e. \<lbrakk>e\<rbrakk>\<^bsub>\<lbrace>h\<rbrace>\<rho>\<^esub>))"
-    unfolding HSem_def'
-    by (rule fix_on_eq[OF fix_on_cond_HSem])  
+    unfolding UHSem_def'
+    by (rule fix_on_eq[OF fix_on_cond_UHSem])  
   
-  lemma the_lookup_HSem_other:
+  lemma the_lookup_UHSem_other:
     assumes "y \<notin> heapVars h"
     shows "(\<lbrace>h\<rbrace>\<rho>) f! y = \<rho> f! y"
-    apply (subst HSem_eq)
+    apply (subst UHSem_eq)
     using assms by simp
 
-  lemma fmap_lookup_bot_HSem_other:
+  lemma fmap_lookup_bot_UHSem_other:
     assumes "y \<notin> heapVars h"
     shows "(\<lbrace>h\<rbrace>\<rho>) f!\<^sub>\<bottom> y = \<rho> f!\<^sub>\<bottom> y"
     using assms
-    by (subst HSem_eq, cases "y \<in> fdom \<rho>", auto)
+    by (subst UHSem_eq, cases "y \<in> fdom \<rho>", auto)
   
-  lemma the_lookup_HSem_heap:
+  lemma the_lookup_UHSem_heap:
     assumes "y \<in> heapVars h"
     shows "(\<lbrace>h\<rbrace>\<rho>) f! y = \<lbrakk> the (map_of h y) \<rbrakk>\<^bsub>\<lbrace>h\<rbrace>\<rho>\<^esub>"
-    apply (subst HSem_eq)
+    apply (subst UHSem_eq)
     using assms by (simp add: lookupHeapToEnv)
 
-  lemma fdom_HSem[simp]:
+  lemma fdom_UHSem[simp]:
     "fdom (\<lbrace>h\<rbrace>\<rho>) = fdom \<rho> \<union> heapVars h"
-    by (subst HSem_eq, simp)
+    by (subst UHSem_eq, simp)
 
   lemma fmap_restr_fmap_addI:"finite S \<Longrightarrow> fdom \<rho>1 - fdom \<rho>2 \<subseteq> S \<Longrightarrow> fmap_restr S \<rho>1 f++ \<rho>2 = \<rho>1 f++ \<rho>2"
     apply (rule fmap_eqI)
@@ -172,63 +170,63 @@ subsubsection {* Induction and other lemmas about @{term HSem} *}
     apply auto
     by (metis lookup_fmap_add1 lookup_fmap_add2 lookup_fmap_restr)
 
-  lemma HSem_restr:
+  lemma UHSem_restr:
     "\<lbrace>h\<rbrace>(fmap_restr (fdom \<rho> - heapVars h) \<rho>) = \<lbrace>h\<rbrace>\<rho>"
-    apply (rule parallel_HSem_ind)
+    apply (rule parallel_UHSem_ind)
     apply simp
     apply auto
     apply (subst fmap_restr_fmap_addI)
     apply simp_all
     done
   
-  lemma HSem_reorder:
+  lemma UHSem_reorder:
     assumes "map_of \<Gamma> = map_of \<Delta>"
     shows "\<lbrace>\<Gamma>\<rbrace>\<rho> = \<lbrace>\<Delta>\<rbrace>\<rho>"
-  by (simp add: HSem_def' heapToEnv_reorder[OF assms] assms dom_map_of_conv_heapVars[symmetric])
+  by (simp add: UHSem_def' heapToEnv_reorder[OF assms] assms dom_map_of_conv_heapVars[symmetric])
   
-  lemma HSem_reorder_head:
+  lemma UHSem_reorder_head:
     assumes "x \<noteq> y"
     shows "\<lbrace>(x,e1)#(y,e2)#\<Gamma>\<rbrace>\<rho> = \<lbrace>(y,e2)#(x,e1)#\<Gamma>\<rbrace>\<rho>"
   proof-
     have "set ((x,e1)#(y,e2)#\<Gamma>) = set ((y,e2)#(x,e1)#\<Gamma>)"
       by auto
     thus ?thesis      
-      unfolding HSem_def  heapToEnv_reorder_head[OF assms]
+      unfolding UHSem_def heapToEnv_reorder_head[OF assms]
       by (simp add: heapVars_def)
   qed
   
-  lemma HSem_reorder_head_append:
+  lemma UHSem_reorder_head_append:
     assumes "x \<notin> heapVars \<Gamma>"
     shows "\<lbrace>(x,e)#\<Gamma>@\<Delta>\<rbrace>\<rho> = \<lbrace>\<Gamma> @ ((x,e)#\<Delta>)\<rbrace>\<rho>"
   proof-
     have "set ((x,e)#\<Gamma>@\<Delta>) = set (\<Gamma> @ ((x,e)#\<Delta>))" by auto
     thus ?thesis
-      unfolding HSem_def  heapToEnv_reorder_head_append[OF assms]
-      by (simp add: )
+      unfolding UHSem_def  heapToEnv_reorder_head_append[OF assms]
+      by simp
   qed  
     
-  lemma fmap_restr_HSem_noop:
+  lemma fmap_restr_UHSem_noop:
     assumes "heapVars \<Gamma> \<inter> fdom \<rho> = {}"
     shows "fmap_restr (fdom \<rho>) (\<lbrace>\<Gamma>\<rbrace>\<rho>) = \<rho>"
     apply (rule fmap_eqI)
     using assms apply auto[1]
     using assms apply auto[1]
-    apply (subst the_lookup_HSem_other)
+    apply (subst the_lookup_UHSem_other)
     apply auto
     done
   
-  lemma HSem_disjoint_less:
+  lemma UHSem_disjoint_less:
     assumes "heapVars \<Gamma> \<inter> fdom \<rho> = {}"
     shows "\<rho> \<le> \<lbrace>\<Gamma>\<rbrace>\<rho>"
     using assms
-  by (metis fmap_less_restrict fmap_restr_HSem_noop)
+  by (metis fmap_less_restrict fmap_restr_UHSem_noop)
 
-  lemma HSem_Nil[simp]: "\<lbrace>[]\<rbrace>\<rho> = \<rho>"
-    by (subst HSem_eq, simp)
+  lemma UHSem_Nil[simp]: "\<lbrace>[]\<rbrace>\<rho> = \<rho>"
+    by (subst UHSem_eq, simp)
 
 subsubsection {* Iterative definition of the heap semantics *}
 
-  lemma iterative_HSem:
+  lemma iterative_UHSem:
     assumes "x \<notin> heapVars \<Gamma>"
     shows "\<lbrace>(x,e) # \<Gamma>\<rbrace>\<rho> =
          fix_on' (f\<emptyset>\<^bsub>[insert x (fdom \<rho> \<union> heapVars \<Gamma>)]\<^esub>)
@@ -246,16 +244,16 @@ subsubsection {* Iterative definition of the heap semantics *}
       by (simp_all add: ESem_cont)
 
     have "\<lbrace>(x,e) # \<Gamma>\<rbrace>\<rho> = fix_on' b L"
-      by (simp add: HSem_def' fmap_add_upd)
+      by (simp add: UHSem_def' fmap_add_upd)
     also have "\<dots> = fix_on' b R"
       by (rule iterative_fmap_add)
     also have "\<dots> = fix_on' (f\<emptyset>\<^bsub>[insert x (fdom \<rho> \<union> heapVars \<Gamma>)]\<^esub>)
             (\<lambda> \<rho>'. (\<rho> f++ fmap_restr (heapVars \<Gamma>) (\<lbrace>\<Gamma>\<rbrace>\<rho>'))( x f\<mapsto> \<lbrakk>e\<rbrakk>\<^bsub>\<rho>'\<^esub>))"
-      by (rule fix_on_cong[OF condR], simp add: HSem_def')
+      by (rule fix_on_cong[OF condR], simp add: UHSem_def')
     finally show ?thesis.
   qed
 
-  lemma iterative_HSem'_cond:
+  lemma iterative_UHSem'_cond:
     assumes "x \<notin> heapVars \<Gamma>"
     shows "fix_on_cond {\<rho>'. f\<emptyset>\<^bsub>[insert x (fdom \<rho> \<union> heapVars \<Gamma>)]\<^esub> \<sqsubseteq> \<rho>'}
              (f\<emptyset>\<^bsub>[insert x (fdom \<rho> \<union> heapVars \<Gamma>)]\<^esub>)
@@ -273,10 +271,10 @@ subsubsection {* Iterative definition of the heap semantics *}
       by (simp_all add: ESem_cont)
 
     show ?thesis
-      by (rule fix_on_cond_cong[OF condR'], simp add: HSem_def')
+      by (rule fix_on_cond_cong[OF condR'], simp add: UHSem_def')
   qed
 
-  lemma iterative_HSem':
+  lemma iterative_UHSem':
     assumes "x \<notin> heapVars \<Gamma>"
     shows "fix_on' (f\<emptyset>\<^bsub>[insert x (fdom \<rho> \<union> heapVars \<Gamma>)]\<^esub>)
             (\<lambda> \<rho>'. (\<rho> f++ fmap_restr (heapVars \<Gamma>) (\<lbrace>\<Gamma>\<rbrace>\<rho>'))( x f\<mapsto> \<lbrakk>e\<rbrakk>\<^bsub>\<rho>'\<^esub>)) 
@@ -297,30 +295,30 @@ subsubsection {* Iterative definition of the heap semantics *}
     have "fix_on' (f\<emptyset>\<^bsub>[insert x (fdom \<rho> \<union> heapVars \<Gamma>)]\<^esub>)
             (\<lambda> \<rho>'. (\<rho> f++ fmap_restr (heapVars \<Gamma>) (\<lbrace>\<Gamma>\<rbrace>\<rho>'))( x f\<mapsto> \<lbrakk>e\<rbrakk>\<^bsub>\<rho>'\<^esub>)) =
           fix_on' b R"
-      by (rule fix_on_cong[symmetric, OF condR], simp add: HSem_def')
+      by (rule fix_on_cong[symmetric, OF condR], simp add: UHSem_def')
     also have "\<dots> = fix_on' b L"
       by (rule iterative_fmap_add[symmetric])
     also have "\<dots> = fix_on' b R'"
       by (rule iterative_fmap_add')
     also have "\<dots> = fix_on' (f\<emptyset>\<^bsub>[insert x (fdom \<rho> \<union> heapVars \<Gamma>)]\<^esub>)
             (\<lambda> \<rho>'. (\<rho> f++ fmap_restr (heapVars \<Gamma>) (\<lbrace>\<Gamma>\<rbrace>\<rho>'))( x f\<mapsto> \<lbrakk>e\<rbrakk>\<^bsub>\<lbrace>\<Gamma>\<rbrace>\<rho>'\<^esub>))"
-      by (rule fix_on_cong[OF condR'], simp add: HSem_def')
+      by (rule fix_on_cong[OF condR'], simp add: UHSem_def')
     finally
     show ?thesis.
   qed
 
 end
 
-lemma HSem_cong[fundef_cong]:
+lemma UHSem_cong[fundef_cong]:
   "\<lbrakk> (\<And> e. e \<in> snd ` set heap2 \<Longrightarrow> ESem1 e = ESem2 e); env1 = env2 ; heap1 = heap2  \<rbrakk>
-      \<Longrightarrow> has_ESem.HSem ESem1 heap1 env1 = has_ESem.HSem  ESem2 heap2 env2"
-  unfolding has_ESem.HSem_def
+      \<Longrightarrow> has_ESem.UHSem ESem1 heap1 env1 = has_ESem.UHSem  ESem2 heap2 env2"
+  unfolding has_ESem.UHSem_def
   by (auto cong:heapToEnv_cong)
 
 subsubsection {* Equivariance *}
 
-lemma HSem_eqvt[eqvt]:
-  "\<pi> \<bullet> has_ESem.HSem ESem h \<rho> = has_ESem.HSem (\<pi> \<bullet> ESem) (\<pi> \<bullet> h) (\<pi> \<bullet> \<rho>)"
+lemma UHSem_eqvt[eqvt]:
+  "\<pi> \<bullet> has_ESem.UHSem ESem h \<rho> = has_ESem.UHSem (\<pi> \<bullet> ESem) (\<pi> \<bullet> h) (\<pi> \<bullet> \<rho>)"
 proof(cases "\<forall> e \<in> snd ` set h.  cont (ESem e)")
 case True
   from permute_boolI[OF this, where p = \<pi>]
@@ -328,8 +326,8 @@ case True
     by perm_simp
 
   show ?thesis          
-   unfolding has_ESem.HSem_def if_P[OF True]  if_P[OF True_permuted] 
-   apply (subst fix_on_eqvt[OF has_ESem.fix_on_cond_HSem'])
+   unfolding has_ESem.UHSem_def if_P[OF True]  if_P[OF True_permuted] 
+   apply (subst fix_on_eqvt[OF has_ESem.fix_on_cond_UHSem'])
    apply (metis True)
    apply perm_simp
    apply rule
@@ -340,7 +338,7 @@ case False
   have False_permuted: "\<not> (\<forall> e \<in> snd ` set (\<pi> \<bullet> h). cont ((\<pi> \<bullet> ESem) e))"
     by perm_simp
   show ?thesis
-   unfolding has_ESem.HSem_def if_not_P[OF False]  if_not_P[OF False_permuted] 
+   unfolding has_ESem.UHSem_def if_not_P[OF False]  if_not_P[OF False_permuted] 
    apply perm_simp
    apply rule
    done
