Launchbury/HasESem.thy
@@ -1,0 +1,12 @@
+theory HasESem
+imports "Nominal-HOLCF" "FMap-HOLCF" "HOLCF-Join"
+begin
+
+locale has_ESem =
+  fixes ESem :: "'exp::pt \<Rightarrow> 'var::{cont_pt,at_base} f\<rightharpoonup> 'value \<Rightarrow> 'value::{pure_cpo,Nonempty_Meet_cpo,pcpo}"  ("\<lbrakk> _ \<rbrakk>\<^bsub>_\<^esub>"  [60,60] 60)
+
+locale has_cont_ESem = has_ESem +
+  assumes ESem_cont: "\<And> e. cont (ESem e)"
+
+
+end
